Tapir modelling

txn-data-consistency/Tapir.thy
@@ -35,210 +35,162 @@ subsection \<open>Event System\<close>
 subsubsection \<open>State\<close>
 
 type_synonym tstmp = nat
-datatype state_svr = idle | try_prep tstmp | occ_s | occ_f | committed | aborted
-datatype state_cl = cl_init | cl_prepared tstmp | cl_committed tstmp | cl_aborted
+
+datatype 'v cl_state =
+  cl_init
+  | cl_prepared tstmp "key set" "key \<rightharpoonup> 'v \<times> txid" "key \<rightharpoonup> 'v"
+  | cl_committed tstmp "key \<rightharpoonup> 'v \<times> txid" "key \<rightharpoonup> 'v"
+  | cl_aborted
+
+datatype 'v svr_state =
+  idle
+  | prep "('v \<times> txid) option" "'v option"
+  | occ_s "('v \<times> txid) option" "'v option"
+  | occ_f
+  | committed_wr (v_val: 'v) "txid0 set" (v_ts: tstmp)
+  | committed_rd 'v txid
+  | aborted
 
 \<comment>\<open>Client State\<close>
-record cl_conf =
-  cl_state :: state_cl
+record 'v cl_conf =
+  cl_state :: "'v cl_state"
   cl_sn :: nat
   cl_view :: view
+  cl_local_time :: tstmp
 
 \<comment>\<open>Server State\<close>
-type_synonym 'v key_fp_ts = "op_type \<rightharpoonup> 'v \<times> tstmp"
-record 'v version_t = "'v version" + v_ts :: tstmp
+type_synonym 'v txn_state = "txid \<Rightarrow> 'v svr_state"
 
 record 'v svr_conf =
-  svr_state :: "txid0 \<Rightarrow> state_svr"
-  svr_vl :: "'v version_t list" \<comment> \<open>not ordered by ts; ts is accessible by v_ts\<close>
-  svr_fp :: "txid0 \<Rightarrow> 'v key_fp_ts"
+  svr_state :: "'v txn_state"
+  svr_ver_order :: "txid list"
   svr_prep_reads :: "txid0 \<rightharpoonup> tstmp"
   svr_prep_writes :: "txid0 \<rightharpoonup> tstmp"
+  (* (txid0 \<rightharpoonup> tstmp \<equiv> (txid0 \<times> tstmp) set) where we know there is only one ts per txid *)
 
 \<comment>\<open>System Global State: Clients and key Servers\<close>
 record 'v global_conf =
-  cls :: "cl_id \<Rightarrow> cl_conf"
+  cls :: "cl_id \<Rightarrow> 'v cl_conf"
   svrs :: "key \<Rightarrow> 'v svr_conf"
+  commit_order :: "key \<Rightarrow> txid list"
+
 
 \<comment> \<open>Translator and helper functions\<close>
 
-abbreviation get_txn :: "cl_id \<Rightarrow> 'v global_conf \<Rightarrow> txid0" where
-  "get_txn cl s \<equiv> Tn_cl (cl_sn (cls s cl)) cl"
+fun get_cl_w :: "txid \<Rightarrow> cl_id" where
+  "get_cl_w T0 = undefined" |
+  "get_cl_w (Tn (Tn_cl sn cl)) = cl"
 
-abbreviation get_fp :: "(txid0 \<Rightarrow> 'v key_fp_ts) \<Rightarrow> txid0 \<Rightarrow> 'v key_fp" where
-  "get_fp svrfp \<equiv> (\<lambda>t op. map_option fst (svrfp t op))"
+abbreviation get_txn :: "'v global_conf \<Rightarrow> cl_id \<Rightarrow> txid0" where
+  "get_txn s cl \<equiv> Tn_cl (cl_sn (cls s cl)) cl"
 
-abbreviation get_ver :: "'v version_t \<Rightarrow> 'v version" where
-  "get_ver v \<equiv> \<lparr> v_value = v_value v, v_writer = v_writer v, v_readerset = v_readerset v\<rparr>"
+abbreviation get_wtxn :: "'v global_conf \<Rightarrow> cl_id \<Rightarrow> txid" where
+  "get_wtxn s cl \<equiv> Tn (get_txn s cl)"
 
-abbreviation read_set :: "('v, 'm) global_conf_scheme \<Rightarrow> txid0 \<Rightarrow> key \<rightharpoonup> ('v \<times> tstmp)" where
-  "read_set s t \<equiv> (\<lambda>k. svr_fp (svrs s k) t R)"
+fun ver_tstmp :: "(txid \<Rightarrow> 'v svr_state) \<Rightarrow> txid \<Rightarrow> tstmp \<times> cl_id"  where
+  "ver_tstmp wtxns t = (v_ts (wtxns t), case t of T0 \<Rightarrow> 0 | Tn t \<Rightarrow> Suc (get_cl t))"
 
-abbreviation write_set :: "('v, 'm) global_conf_scheme \<Rightarrow> txid0 \<Rightarrow> key \<rightharpoonup> ('v \<times> tstmp)" where
-  "write_set s t \<equiv> (\<lambda>k. svr_fp (svrs s k) t W)"
-
-fun ver_tstmp where
-  "ver_tstmp ver = (v_ts ver, case v_writer ver of T0 \<Rightarrow> 0 | Tn t \<Rightarrow> Suc (get_cl t))"
-
-abbreviation new_vers_t :: "txid \<Rightarrow> 'v \<Rightarrow> tstmp \<Rightarrow> 'v version_t" where
-  "new_vers_t t v ts \<equiv> \<lparr>v_value = v, v_writer = t, v_readerset = {}, v_ts = ts\<rparr>"
-
-fun update_kv_key_writes_t :: "txid0 \<Rightarrow> 'v option \<Rightarrow> tstmp \<Rightarrow> 'v version_t list \<Rightarrow> 'v version_t list" where
-  "update_kv_key_writes_t t None ts vl = vl" |
-  "update_kv_key_writes_t t (Some v) ts vl = vl @ [new_vers_t (Tn t) v ts]"
-
-definition update_kv_key_t :: "txid0 \<Rightarrow> 'v key_fp \<Rightarrow> tstmp \<Rightarrow> key_view \<Rightarrow> 'v version_t list \<Rightarrow> 'v version_t list" where
-  "update_kv_key_t t Fk ts uk = update_kv_key_writes_t t (Fk W) ts o update_kv_key_reads t (Fk R) uk"
+definition add_to_readerset :: "'v txn_state \<Rightarrow> txid0 \<Rightarrow> txid \<Rightarrow> 'v txn_state" where
+  "add_to_readerset wtxns t t_wr \<equiv> (case wtxns t_wr of
+    committed_wr v rs ts \<Rightarrow>
+      wtxns (Tn t := committed_rd v t_wr, t_wr := committed_wr v (insert t rs) ts) |
+    _ \<Rightarrow> wtxns)"
 
 subsubsection \<open>Simulation function\<close>
+definition ready_to_commit_reads where
+  "ready_to_commit_reads s t_wr \<equiv> {t_rd. \<exists>ts r_map w_map k v.
+    cl_state (cls s (get_cl t_rd)) = cl_committed ts r_map w_map \<and>
+    svr_state (svrs s k) (Tn t_rd) = occ_s (Some (v, t_wr)) None}"
 
-definition eligible_reads :: "(txid0 \<Rightarrow> state_cl) \<Rightarrow> (txid0 \<Rightarrow> state_svr) \<Rightarrow>
-  (txid0 \<Rightarrow> 'v key_fp) \<Rightarrow> txid0 set" where
-  "eligible_reads tCls tSvrs tFk \<equiv> {t.
-     \<exists>ts. tCls t = cl_committed ts \<and> tSvrs t \<in> {occ_s} \<and> tFk t R \<noteq> None}"
+definition txn_to_vers :: "('v, 'm) global_conf_scheme \<Rightarrow> key \<Rightarrow> txid \<Rightarrow> 'v version" where
+  "txn_to_vers s k = (\<lambda>t. case svr_state (svrs s k) t of
+    occ_s None (Some v) \<Rightarrow> \<lparr>v_value = v, v_writer = t, v_readerset = {}\<rparr> |
+    committed_wr v rs ts \<Rightarrow> \<lparr>v_value = v, v_writer = t, v_readerset = rs \<union> ready_to_commit_reads s t\<rparr>)"
 
-definition update_kv_key_reads_all_txn :: "(txid0 \<Rightarrow> state_cl) \<Rightarrow> (txid0 \<Rightarrow> state_svr) \<Rightarrow>
-  (txid0 \<Rightarrow> 'v key_fp) \<Rightarrow> 'v v_list \<Rightarrow> 'v v_list" where
-  "update_kv_key_reads_all_txn tCls tSvrs tFk vl =
-    (let uk = full_view vl; lv = last_version vl uk in
-     vl [Max uk := lv \<lparr>v_readerset := (v_readerset lv) \<union> eligible_reads tCls tSvrs tFk\<rparr>])"
+definition kvs_of_s :: "'v global_conf \<Rightarrow> 'v kv_store" where
+  "kvs_of_s s \<equiv> (\<lambda>k. map (txn_to_vers s k) (commit_order s k))"
 
-abbreviation the_wr_t :: "(txid0 \<Rightarrow> state_svr) \<Rightarrow> txid0" where
-  "the_wr_t tSvrs \<equiv> (THE t. tSvrs t = occ_s)"
+lemmas kvs_of_s_defs = kvs_of_s_def txn_to_vers_def ready_to_commit_reads_def
 
-definition update_kv_key_writes_all_txn :: "(txid0 \<Rightarrow> state_cl) \<Rightarrow> (txid0 \<Rightarrow> state_svr) \<Rightarrow>
-  (txid0 \<Rightarrow> 'v key_fp) \<Rightarrow> 'v v_list \<Rightarrow> 'v v_list" where
-  "update_kv_key_writes_all_txn tCls tSvrs tFk vl =
-    (if (\<exists>t ts. tCls t = cl_committed ts \<and> tSvrs t = occ_s) then
-        update_kv_key_writes (the_wr_t tSvrs) (tFk (the_wr_t tSvrs) W) vl
-     else vl)"
-
-definition update_kv_all_txn :: "(txid0 \<Rightarrow> state_cl) \<Rightarrow> (txid0 \<Rightarrow> state_svr) \<Rightarrow>
-  (txid0 \<Rightarrow> 'v key_fp) \<Rightarrow> 'v v_list \<Rightarrow> 'v v_list" where
-  "update_kv_all_txn tCls tSvrs tFk =
-    (update_kv_key_writes_all_txn tCls tSvrs tFk) o (update_kv_key_reads_all_txn tCls tSvrs tFk)"
-
-definition kvs_of_gs :: "'v global_conf \<Rightarrow> 'v kv_store" where
-  "kvs_of_gs gs = (\<lambda>k.
-   update_kv_all_txn (\<lambda>t. cl_state (cls gs (get_cl t)))
-    (svr_state (svrs gs k)) (get_fp (svr_fp (svrs gs k))) (map get_ver (svr_vl (svrs gs k))))"
-
-definition views_of_gs :: "'v global_conf \<Rightarrow> (cl_id \<Rightarrow> view)" where
-  "views_of_gs gs = (\<lambda>cl. cl_view (cls gs cl))"
+definition views_of_s :: "'v global_conf \<Rightarrow> (cl_id \<Rightarrow> view)" where
+  "views_of_s gs = (\<lambda>cl. cl_view (cls gs cl))"
 
 definition sim :: "'v global_conf \<Rightarrow> 'v config" where         
-  "sim gs = (kvs_of_gs gs, views_of_gs gs)"
+  "sim gs = (kvs_of_s gs, views_of_s gs)"
 
-lemmas update_kv_key_reads_all_defs = update_kv_key_reads_all_txn_def Let_def 
-lemmas update_kv_all_defs = update_kv_key_reads_all_defs update_kv_key_writes_all_txn_def update_kv_all_txn_def
-lemmas sim_defs = sim_def kvs_of_gs_def views_of_gs_def
+lemmas sim_defs = sim_def kvs_of_s_defs views_of_s_def
 
 
 subsubsection \<open>Events\<close>
 
-datatype 'v ev = TryPrep key txid0 tstmp | OCCCheck key txid0 tstmp | Commit key txid0 tstmp | Abort key txid0 |
-  Cl_Prep cl_id tstmp | Cl_Commit cl_id sqn view "'v fingerpr" tstmp | Cl_Abort cl_id | Cl_ReadyC cl_id |
-  Cl_ReadyA cl_id | Skip2
+datatype 'v ev =
+    Cl_Prep cl_id tstmp "key set" "key \<rightharpoonup> 'v"
+  | Cl_Read_Resp cl_id key 'v txid
+  | Cl_Commit cl_id sqn view "'v fingerpr" tstmp "key \<rightharpoonup> ('v \<times> txid)" "key \<rightharpoonup> 'v"
+  | Cl_Abort cl_id
+  | Cl_ReadyC cl_id tstmp
+  | Cl_ReadyA cl_id tstmp
+  | Prep key txid0 "('v \<times> txid) option" "'v option"
+  | OCCCheck key txid0 tstmp "('v \<times> txid) option" "'v option" "'v svr_state"
+  | CommitW key 'v txid0 tstmp
+  | CommitR key 'v txid txid0
+  | Abort key txid0
+  | Skip2
 
 abbreviation is_curr_t :: "('v, 'm) global_conf_scheme \<Rightarrow> txid0 \<Rightarrow> bool" where
   "is_curr_t s t \<equiv> cl_sn (cls s (get_cl t)) = get_sn t"
 
-definition updated_kvs :: "'v global_conf \<Rightarrow> cl_id \<Rightarrow> tstmp \<Rightarrow> 'v kv_store" where
-  "updated_kvs s cl ts \<equiv> (\<lambda>k. update_kv_all_txn
-    (\<lambda>t. cl_state (cls (s \<lparr> cls := (cls s)
-      (cl := cls s cl \<lparr> cl_state := cl_committed ts \<rparr> ) \<rparr>) (get_cl t)))
-    (svr_state (svrs s k)) (get_fp (svr_fp (svrs s k))) (map get_ver (svr_vl (svrs s k))))"
-
-definition prepare where
-  "prepare k t ts s s' \<equiv>
-    is_curr_t s t \<and>
-    cl_state (cls s (get_cl t)) = cl_prepared ts \<and>
-    svr_state (svrs s k) t = idle \<and>
-    s' = s \<lparr> svrs := (svrs s)
-      (k := svrs s k \<lparr>
-        svr_state := (svr_state (svrs s k)) (t := try_prep ts)
-      \<rparr>)
-    \<rparr>"
-
-definition occ_check :: "key \<Rightarrow> txid0 \<Rightarrow> tstmp \<Rightarrow> ('v, 'm) global_conf_scheme \<Rightarrow> state_svr" where
-  "occ_check k t ts s =
-    (let prep_rd_ts = {(ts', Suc (get_cl t')) | t' ts'. svr_prep_reads (svrs s k) t' = Some ts'};
-        prep_wr_ts = {(ts', Suc (get_cl t')) | t' ts'. svr_prep_writes (svrs s k) t' = Some ts'} in
-    (if (\<exists>ver_v ver_ts. read_set s t k = Some (ver_v, ver_ts) \<and>
-         (ver_ts, Suc (get_cl t)) < Max {ver_tstmp ver | ver. ver \<in> set (svr_vl (svrs s k))})
-     then occ_f
-     else (
-      if (k \<in> dom (read_set s t) \<and> prep_wr_ts \<noteq> {} \<and> (ts, Suc (get_cl t)) > Min prep_wr_ts)
-      then occ_f
-      else (
-        if (k \<in> dom (write_set s t) \<and> prep_rd_ts \<noteq> {} \<and> (ts, Suc (get_cl t)) < Max prep_rd_ts)
-        then occ_f
-        else (
-          if (k \<in> dom (write_set s t) \<and> (ts, Suc (get_cl t)) < Max {ver_tstmp ver | ver. ver \<in> set (svr_vl (svrs s k))})
-          then occ_f
-          else occ_s)))))"
-
-definition tapir_occ_check :: "key \<Rightarrow> txid0 \<Rightarrow> tstmp \<Rightarrow> ('v, 'm) global_conf_scheme \<Rightarrow> ('v, 'm) global_conf_scheme \<Rightarrow> bool" where
-  "tapir_occ_check k t ts s s' \<equiv>
-    is_curr_t s t \<and>
-    svr_state (svrs s k) t = try_prep ts \<and>
-    s' = s \<lparr> svrs := (svrs s) (k := svrs s k \<lparr>
-      svr_state := (svr_state (svrs s k)) (t := occ_check k t ts s)
-      \<rparr>)
-    \<rparr>"
-
-definition commit where
-  "commit k t ts s s' \<equiv>
-    is_curr_t s t \<and>
-    cl_state (cls s (get_cl t)) = cl_committed ts \<and>
-    svr_state (svrs s k) t = occ_s \<and>
-    s' = s \<lparr> svrs := (svrs s)
-      (k := svrs s k \<lparr>
-        svr_vl :=
-          update_kv_key_t t (get_fp (svr_fp (svrs s k)) t) ts (full_view (svr_vl (svrs s k))) (svr_vl (svrs s k)),
-        svr_state := (svr_state (svrs s k)) (t := committed)
-      \<rparr>)
-    \<rparr>"
-
-definition abort where
-  "abort k t s s' \<equiv>
-    is_curr_t s t \<and>
-    cl_state (cls s (get_cl t)) = cl_aborted \<and>
-    svr_state (svrs s k) t \<in> {occ_s, occ_f} \<and>
-    s' = s \<lparr> svrs := (svrs s)
-      (k := svrs s k \<lparr>
-        svr_state := (svr_state (svrs s k)) (t := aborted)
-      \<rparr>)
-    \<rparr>"
-
 definition cl_prepare where
-  "cl_prepare cl ts s s' \<equiv> \<comment> \<open>The timestamp ts is proposed by the client\<close>
+  "cl_prepare cl ts r_set w_map s s' \<equiv>
     cl_state (cls s cl) = cl_init \<and>
+    ts = cl_local_time (cls s cl) \<and>  \<comment> \<open>The timestamp ts is proposed by the client\<close>
+    r_set \<inter> dom w_map = {} \<and>
+    (r_set \<noteq> {} \<or> dom w_map \<noteq> {}) \<and>
     s' = s \<lparr> cls := (cls s)
       (cl := cls s cl \<lparr>
-        cl_state := cl_prepared ts \<comment> \<open>The proposed ts is sent to the servers\<close>
+        cl_state := cl_prepared ts r_set (Map.empty) w_map
+        \<comment> \<open>The proposed ts, read set, and write map of the transaction is sent to the servers\<close>
+      \<rparr>)
+    \<rparr>"
+
+definition cl_read_resp where
+  "cl_read_resp cl k v t_wr s s' \<equiv>
+    (\<exists>ts r_set r_map w_map. cl_state (cls s cl) = cl_prepared ts r_set r_map w_map \<and>
+      k \<in> r_set \<and> r_map k = None) \<and>
+    svr_state (svrs s k) (get_wtxn s cl) = prep (Some (v, t_wr)) None \<and>
+    s' = s \<lparr> cls := (cls s)
+      (cl := cls s cl \<lparr>
+        cl_state := case cl_state (cls s cl) of
+                    cl_prepared ts r_set r_map w_map \<Rightarrow>
+                    cl_prepared ts r_set (r_map (k \<mapsto> (v, t_wr))) w_map
       \<rparr>)
     \<rparr>"
 
 definition cl_commit where
-  "cl_commit cl sn u'' F ts s s' \<equiv>
+  "cl_commit cl sn u'' F ts r_map w_map s s' \<equiv>
     sn = cl_sn (cls s cl) \<and>
-    u'' = full_view o (kvs_of_gs s) \<and>
-    F = (\<lambda>k. get_fp (svr_fp (svrs s k)) (get_txn cl s)) \<and>
-    cl_state (cls s cl) = cl_prepared ts \<and>
-    (\<forall>k. svr_state (svrs s k) (get_txn cl s) = occ_s) \<and>
+    u'' = full_view o (kvs_of_s s) \<and>
+    cl_state (cls s cl) = cl_prepared ts (dom r_map) r_map w_map \<and>
+    (\<forall>k \<in> dom r_map \<union> dom w_map. \<exists>r_vto w_vo.
+      svr_state (svrs s k) (get_wtxn s cl) = occ_s r_vto w_vo \<and> 
+      F k R = map_option fst r_vto \<and>
+      F k W = w_vo) \<and>
+    (\<forall>k. k \<notin> dom r_map \<union> dom w_map \<longrightarrow> F k = Map.empty) \<and>
     s' = s \<lparr> cls := (cls s)
       (cl := cls s cl \<lparr>
-        cl_state := cl_committed ts,
-        cl_view := full_view o (updated_kvs s cl ts)
-      \<rparr>)
+        cl_state := cl_committed ts r_map w_map,
+        cl_view := full_view o (kvs_of_s s')
+      \<rparr>),
+      commit_order := (\<lambda>k. if w_map k = None then commit_order s k else commit_order s k @ [get_wtxn s cl])
     \<rparr>"
 
 definition cl_abort where
   "cl_abort cl s s' \<equiv>
-    (\<exists>ts. cl_state (cls s cl) = cl_prepared ts) \<and>
-    (\<exists>k. svr_state (svrs s k) (get_txn cl s) = occ_f) \<and>
-    (\<forall>k. svr_state (svrs s k) (get_txn cl s) \<in> {occ_s, occ_f}) \<and>
+    (\<exists>ts r_map w_map. cl_state (cls s cl) = cl_prepared ts (dom r_map) r_map w_map \<and>
+    (\<exists>k \<in> dom r_map \<union> dom w_map.
+      svr_state (svrs s k) (get_wtxn s cl) = occ_f) \<and>
+    (\<forall>k \<in> dom r_map \<union> dom w_map.
+      \<exists>r_vto w_vo. svr_state (svrs s k) (get_wtxn s cl) \<in> {occ_s r_vto w_vo, occ_f})) \<and>
     s' = s \<lparr> cls := (cls s)
       (cl := cls s cl \<lparr>
         cl_state := cl_aborted
@@ -246,24 +198,118 @@ definition cl_abort where
     \<rparr>"
 
 definition cl_ready_c where
-  "cl_ready_c cl s s' \<equiv>
-    (\<exists>ts. cl_state (cls s cl) = cl_committed ts) \<and>
-    (\<forall>k. svr_state (svrs s k) (get_txn cl s) = committed) \<and>
+  "cl_ready_c cl clk s s' \<equiv>
+    (\<exists>ts r_map w_map. cl_state (cls s cl) = cl_committed ts r_map w_map \<and>
+      (\<forall>k \<in> dom r_map. \<exists>v t. svr_state (svrs s k) (get_wtxn s cl) = committed_rd v t) \<and>
+      (\<forall>k \<in> dom w_map. \<exists>v. svr_state (svrs s k) (get_wtxn s cl) = committed_wr v {} ts)) \<and>
+    clk > cl_local_time (cls s cl) \<and>
     s' = s \<lparr> cls := (cls s)
       (cl := cls s cl \<lparr>
         cl_state := cl_init,
-        cl_sn := Suc (cl_sn (cls s cl))
+        cl_sn := Suc (cl_sn (cls s cl)),
+        cl_local_time := clk
       \<rparr>)
     \<rparr>"
 
 definition cl_ready_a where
-  "cl_ready_a cl s s' \<equiv>
+  "cl_ready_a cl clk s s' \<equiv>
     cl_state (cls s cl) = cl_aborted \<and>
-    (\<forall>k. svr_state (svrs s k) (get_txn cl s) = aborted) \<and>
+    (\<forall>k. svr_state (svrs s k) (get_wtxn s cl) = aborted) \<and>
+    clk > cl_local_time (cls s cl) \<and>
     s' = s \<lparr> cls := (cls s)
       (cl := cls s cl \<lparr>
         cl_state := cl_init,
-        cl_sn := Suc (cl_sn (cls s cl))
+        cl_sn := Suc (cl_sn (cls s cl)),
+        cl_local_time := clk
+      \<rparr>)
+    \<rparr>"
+
+definition prepare where
+  "prepare k t r_vto w_vo s s' \<equiv>
+    is_curr_t s t \<and>
+    (\<exists>ts r_set r_map w_map. cl_state (cls s (get_cl t)) = cl_prepared ts r_set r_map w_map \<and>
+      ((k \<in> r_set \<and> k \<notin> dom r_map) \<or> k \<in> dom w_map) \<and>
+      r_vto = (if k \<in> r_set
+             then Some ((\<lambda>t. (v_val (svr_state (svrs s k) t), t)) (last (svr_ver_order (svrs s k))))
+             else None) \<and>
+      w_vo = w_map k) \<and>
+    svr_state (svrs s k) (Tn t) = idle \<and>
+    s' = s \<lparr> svrs := (svrs s)
+      (k := svrs s k \<lparr>
+        svr_state := (svr_state (svrs s k)) (Tn t := prep r_vto w_vo)
+      \<rparr>)
+    \<rparr>"
+
+definition occ_check :: "key \<Rightarrow> txid0 \<Rightarrow> tstmp \<Rightarrow> ('v \<times> txid) option \<Rightarrow> 'v option
+  \<Rightarrow> ('v, 'm) global_conf_scheme \<Rightarrow> 'v svr_state" where
+  "occ_check k t ts r_vto w_vo s =
+    (let prep_rd_ts = {(ts', Suc (get_cl t')) | t' ts'. svr_prep_reads (svrs s k) t' = Some ts'};
+        prep_wr_ts = {(ts', Suc (get_cl t')) | t' ts'. svr_prep_writes (svrs s k) t' = Some ts'} in
+    (if (\<exists>ver_v ver_wr. r_vto = Some (ver_v, ver_wr) \<and>
+         ver_tstmp (svr_state (svrs s k)) ver_wr <
+         Max {ver_tstmp (svr_state (svrs s k)) t_wr | t_wr. t_wr \<in> set (svr_ver_order (svrs s k))})
+     then occ_f
+     else (
+      if (r_vto \<noteq> None \<and> prep_wr_ts \<noteq> {} \<and> (ts, Suc (get_cl t)) > Min prep_wr_ts)
+      then occ_f
+      else (
+        if (w_vo \<noteq> None \<and> prep_rd_ts \<noteq> {} \<and> (ts, Suc (get_cl t)) < Max prep_rd_ts)
+        then occ_f
+        else (
+          if (w_vo \<noteq> None \<and>
+              (ts, Suc (get_cl t)) <
+              Max {ver_tstmp (svr_state (svrs s k)) t_wr | t_wr. t_wr \<in> set (svr_ver_order (svrs s k))})
+          then occ_f
+          else occ_s r_vto w_vo)))))"
+
+definition tapir_occ_check where
+  "tapir_occ_check k t ts r_vto w_vo occ_res s s' \<equiv>
+    is_curr_t s t \<and>
+    (\<exists>r_map w_map. cl_state (cls s (get_cl t)) = cl_prepared ts (dom r_map) r_map w_map) \<and>
+    svr_state (svrs s k) (Tn t) = prep r_vto w_vo \<and>
+    occ_res = occ_check k t ts r_vto w_vo s \<and>
+    s' = s \<lparr> svrs := (svrs s) (k := svrs s k \<lparr>
+      svr_state := (svr_state (svrs s k)) (Tn t := occ_res),
+      svr_prep_reads := if occ_res = occ_f \<or> r_vto = None
+                        then svr_prep_reads (svrs s k)
+                        else (svr_prep_reads (svrs s k)) (t := Some ts),
+      svr_prep_writes := if occ_res = occ_f \<or> w_vo = None
+                         then svr_prep_writes (svrs s k)
+                         else (svr_prep_writes (svrs s k)) (t := Some ts)
+      \<rparr>)
+    \<rparr>"
+
+definition commit_rd where
+  "commit_rd k v t_wr t s s' \<equiv>
+    is_curr_t s t \<and>
+    (\<exists>ts r_map w_map. cl_state (cls s (get_cl t)) = cl_committed ts r_map w_map) \<and>
+    svr_state (svrs s k) (Tn t) = occ_s (Some (v, t_wr)) None \<and>
+    s' = s \<lparr> svrs := (svrs s)
+      (k := svrs s k \<lparr>
+        svr_state := add_to_readerset (svr_state (svrs s k)) t t_wr
+      \<rparr>)                                             
+    \<rparr>"
+
+definition commit_wr where
+  "commit_wr k v t ts s s' \<equiv>
+    is_curr_t s t \<and>
+    (\<exists>r_map w_map. cl_state (cls s (get_cl t)) = cl_committed ts r_map w_map) \<and>
+    svr_state (svrs s k) (Tn t) = occ_s None (Some v) \<and>
+    s' = s \<lparr> svrs := (svrs s)
+      (k := svrs s k \<lparr>
+        svr_state := ((svr_state (svrs s k)) (Tn t := committed_wr v {} ts)),
+        svr_ver_order := svr_ver_order (svrs s k) @ [Tn t]
+      \<rparr>)                                             
+    \<rparr>"
+
+definition abort where
+  "abort k t s s' \<equiv>
+    is_curr_t s t \<and>
+    cl_state (cls s (get_cl t)) = cl_aborted \<and>
+    (\<exists>r_vto w_vo. svr_state (svrs s k) (Tn t) \<in> {occ_s r_vto w_vo, occ_f}) \<and>
+    s' = s \<lparr> svrs := (svrs s)
+      (k := svrs s k \<lparr>
+        svr_state := (svr_state (svrs s k)) (Tn t := aborted)
       \<rparr>)
     \<rparr>"
 
@@ -273,26 +319,29 @@ subsubsection \<open>The Event System\<close>
 definition s_init :: "'v global_conf" where
   "s_init \<equiv> \<lparr> 
     cls = (\<lambda>cl. \<lparr> cl_state = cl_init,
-                 cl_sn = 0,
-                 cl_view = view_init \<rparr>),
-    svrs = (\<lambda>k. \<lparr> svr_state = (\<lambda>t. idle),
-                 svr_vl = [new_vers_t T0 undefined 0],
-                 svr_fp = (\<lambda>t. Map.empty),
-                 svr_prep_reads = Map.empty,
-                 svr_prep_writes = Map.empty\<rparr>)
+                  cl_sn = 0,
+                  cl_view = view_init,
+                  cl_local_time = 0 \<rparr>),
+    svrs = (\<lambda>k. \<lparr> svr_state = (\<lambda>t. idle) (T0 := committed_wr undefined {} 0),
+                  svr_ver_order = [T0],
+                  svr_prep_reads = Map.empty,
+                  svr_prep_writes = Map.empty\<rparr>),
+    commit_order = (\<lambda>k. [T0])
   \<rparr>"
 
 fun s_trans :: "'v global_conf \<Rightarrow> 'v ev \<Rightarrow> 'v global_conf \<Rightarrow> bool" where
-  "s_trans s (TryPrep k t ts)         s' \<longleftrightarrow> prepare k t ts s s'" |
-  "s_trans s (OCCCheck k t ts)        s' \<longleftrightarrow> tapir_occ_check k t ts s s'" |
-  "s_trans s (Commit k t ts)          s' \<longleftrightarrow> commit k t ts s s'" |
-  "s_trans s (Abort k t)              s' \<longleftrightarrow> abort k t s s'" |
-  "s_trans s (Cl_Prep cl ts)          s' \<longleftrightarrow> cl_prepare cl ts s s'" |
-  "s_trans s (Cl_Commit cl sn u F ts) s' \<longleftrightarrow> cl_commit cl sn u F ts s s'" |
-  "s_trans s (Cl_Abort cl)            s' \<longleftrightarrow> cl_abort cl s s'" |
-  "s_trans s (Cl_ReadyC cl)           s' \<longleftrightarrow> cl_ready_c cl s s'" |
-  "s_trans s (Cl_ReadyA cl)           s' \<longleftrightarrow> cl_ready_a cl s s'" |
-  "s_trans s Skip2                    s' \<longleftrightarrow> s' = s"
+  "s_trans s (Cl_Prep cl ts rs wm)            s' \<longleftrightarrow> cl_prepare cl ts rs wm s s'" |
+  "s_trans s (Cl_Read_Resp cl k v t_wr)       s' \<longleftrightarrow> cl_read_resp cl k v t_wr s s'" |
+  "s_trans s (Cl_Commit cl sn u F ts rm wm)   s' \<longleftrightarrow> cl_commit cl sn u F ts rm wm s s'" |
+  "s_trans s (Cl_Abort cl)                    s' \<longleftrightarrow> cl_abort cl s s'" |
+  "s_trans s (Cl_ReadyC cl clk)               s' \<longleftrightarrow> cl_ready_c cl clk s s'" |
+  "s_trans s (Cl_ReadyA cl clk)               s' \<longleftrightarrow> cl_ready_a cl clk s s'" |
+  "s_trans s (Prep k t r_vto w_vo)            s' \<longleftrightarrow> prepare k t r_vto w_vo s s'" |
+  "s_trans s (OCCCheck k t ts r_vto w_vo res) s' \<longleftrightarrow> tapir_occ_check k t ts r_vto w_vo res s s'" |
+  "s_trans s (CommitR k v t_wr t)             s' \<longleftrightarrow> commit_rd k v t_wr t s s'" |
+  "s_trans s (CommitW k v t ts)               s' \<longleftrightarrow> commit_wr k v t ts s s'" |
+  "s_trans s (Abort k t)                      s' \<longleftrightarrow> abort k t s s'" |
+  "s_trans s Skip2                            s' \<longleftrightarrow> s' = s"
 
 definition tapir :: "('v ev, 'v global_conf) ES" where
   "tapir \<equiv> \<lparr>
@@ -300,8 +349,9 @@ definition tapir :: "('v ev, 'v global_conf) ES" where
     trans = s_trans
   \<rparr>"
 
-lemmas tapir_trans_defs = prepare_def tapir_occ_check_def commit_def abort_def
-                        cl_prepare_def cl_commit_def cl_abort_def cl_ready_c_def cl_ready_a_def
+lemmas tapir_trans_defs =
+  cl_prepare_def cl_read_resp_def cl_commit_def cl_abort_def cl_ready_c_def cl_ready_a_def
+  prepare_def tapir_occ_check_def commit_rd_def commit_wr_def abort_def
 
 lemmas tapir_defs = tapir_def s_init_def
 
@@ -310,7 +360,7 @@ lemma tapir_trans [simp]: "trans tapir = s_trans" by (simp add: tapir_def)
 subsubsection \<open>Mediator function\<close>
 
 fun med :: "'v ev \<Rightarrow> 'v label" where
-  "med (Cl_Commit cl sn u'' F ts) = ET cl sn u'' F" |
+  "med (Cl_Commit cl sn u'' F ts rm wm) = ET cl sn u'' F" |
   "med _ = ETSkip"
 
 end
