txn-data-consistency/Tapir_Falsification.thy
@@ -6,46 +6,20 @@ begin
 
 subsection \<open>Lemmas and Invariants\<close>
 
-lemma update_kv_all_txn_v_value_inv:
-  assumes "i \<in> full_view vl"
-  shows "v_value (update_kv_all_txn tStm tSkm tFk vl ! i) = v_value (vl ! i)"
-  using assms
-  by (auto simp add: update_kv_all_defs update_kv_key_writes_simps nth_append full_view_def
-           split: option.split)
+lemma ext_map_neqE:
+  "\<lbrakk>(\<lambda>k. map (\<lambda>t. P k t) (l k)) \<noteq> (\<lambda>k. map (\<lambda>t. Q k t) (l k)); \<exists>k t. P k t \<noteq> Q k t \<Longrightarrow> thesis\<rbrakk> \<Longrightarrow> thesis"
+proof -
+  assume a1: "(\<lambda>k. map (P k) (l k)) \<noteq> (\<lambda>k. map (Q k) (l k))"
+  assume a2: "\<exists>k t. P k t \<noteq> Q k t \<Longrightarrow> thesis"
+  obtain aa :: 'a where
+    "map (P aa) (l aa) \<noteq> map (Q aa) (l aa)"
+    using a1 by metis
+  then show ?thesis
+    using a2 by metis
+qed
 
-lemma update_kv_key_reads_all_txn_length [simp]:
-  "length (update_kv_key_reads_all_txn tStm tSkm tFk vl) = length vl"
-  by (auto simp add: update_kv_key_reads_all_defs)
 
-lemma writer_update_before:
-  assumes "reach tapir s"
-    and "cl_state (cls s cl) = cl_prepared ts"
-    and "svr_state (svrs s k) (get_txn cl s) = occ_s"
-  shows "update_kv_all_txn (\<lambda>t. cl_state (cls s (get_cl t))) (svr_state (svrs s k)) tFk vl =
-         update_kv_key_reads_all_txn (\<lambda>t. cl_state (cls s (get_cl t))) (svr_state (svrs s k)) tFk vl"
-  using assms
-  (*by (auto 4 3 simp add: update_kv_all_defs split: option.split)*) oops
 
-lemma svr_vl_kvs_eq_length:
-  assumes "reach tapir s"
-    and "cl_state (cls s cl) = cl_prepared ts"
-    and "svr_state (svrs s k) (get_txn cl s) = occ_s"
-  shows "length (kvs_of_gs s k) = length (svr_vl (svrs s k))"
-  using assms
-  apply (auto simp add: kvs_of_gs_def update_kv_all_defs)
-  (*by (metis assms(1) update_kv_key_reads_all_txn_length writer_update_before)*) oops
-
-lemma svr_vl_kvs_eq_lv:
-  assumes "reach tapir s"
-    and "cl_state (cls s cl) = cl_prepared ts"
-    and "svr_state (svrs s k) (get_txn cl s) = occ_s"
-  shows "v_value (last_version (kvs_of_gs s k) (full_view (kvs_of_gs s k))) =
-         v_value (last_version (svr_vl (svrs s k)) (full_view (svr_vl (svrs s k))))"
-  using assms (*svr_vl_kvs_eq_length[of s]
-    update_kv_all_txn_v_value_inv[of "Max {..<length (svr_vl (svrs s k))}" "svr_vl (svrs s k)"]
-  apply (auto simp add: full_view_def kvs_of_gs_def KVSNonEmp_def)
-  apply (metis full_view_def lessThan_iff max_in_full_view)
-  by (metis full_view_def lessThan_iff max_in_full_view)*) oops
 
 subsection \<open>Refinement Attempt\<close>
 
@@ -55,31 +29,31 @@ proof (intro simulate_ES_fun)
   assume p: "init tapir gs0"
   then show "init ET_SER.ET_ES (sim gs0)"
     by (auto simp add: ET_SER.ET_ES_defs tapir_defs sim_defs kvs_init_def v_list_init_def 
-                       version_init_def update_kv_all_defs eligible_reads_def)
+                       version_init_def)
 next
   fix gs a and gs' :: "'v global_conf"
   assume p: "tapir: gs\<midarrow>a\<rightarrow> gs'" and reach_s: "reach tapir gs" and "reach ET_SER.ET_ES (sim gs)"
   then have (*I: "invariants_list gs" and *) reach_s': "reach tapir gs'" by auto
   with p show "ET_SER.ET_ES: sim gs\<midarrow>med a\<rightarrow> sim gs'"
   proof (induction a)
-    case (Cl_Commit cl sn u'' F ts)
+    case (Cl_Commit cl sn u'' F ts  r_map w_map)
     show ?case 
     proof -
       { 
-        assume cmt: \<open>cl_commit cl sn u'' F ts gs gs'\<close> (*and I: \<open>invariant_list gs\<close>*)
+        assume cmt: \<open>cl_commit cl sn u'' F ts r_map w_map gs gs'\<close> (*and I: \<open>invariant_list gs\<close>*)
         have \<open>ET_SER.ET_trans_and_fp 
-                (kvs_of_gs gs, views_of_gs gs) (ET cl sn u'' F) (kvs_of_gs gs', views_of_gs gs')\<close>
-        proof (rule ET_SER.ET_trans_rule [where u'="full_view o (updated_kvs gs cl ts)"])
-          show \<open>views_of_gs gs cl \<sqsubseteq> u''\<close> using cmt (* I
+                (kvs_of_s gs, views_of_s gs) (ET cl sn u'' F) (kvs_of_s gs', views_of_s gs')\<close>
+        proof (rule ET_SER.ET_trans_rule [where u'="full_view o (kvs_of_s gs')"])
+          show \<open>views_of_s gs cl \<sqsubseteq> u''\<close> using cmt (* I
             apply (auto 4 3 simp add: cl_commit_def views_of_gs_def)*) sorry
         next 
-          show \<open>ET_SER.canCommit (kvs_of_gs gs) u'' F\<close> using cmt (* I 
+          show \<open>ET_SER.canCommit (kvs_of_s gs) u'' F\<close> using cmt (* I 
             by (auto simp add: cl_commit_def full_view_satisfies_ET_SER_canCommit)*) sorry
         next 
-          show \<open>view_wellformed (kvs_of_gs gs) u''\<close> using cmt (* I
+          show \<open>view_wellformed (kvs_of_s gs) u''\<close> using cmt (* I
             by (auto 4 4 simp add: cl_commit_def full_view_wellformed)*) sorry
         next 
-          show \<open>view_wellformed (kvs_of_gs gs') (full_view o (updated_kvs gs cl ts))\<close> using cmt (*I
+          show \<open>view_wellformed (kvs_of_s gs') (full_view o (kvs_of_s gs'))\<close> using cmt (*I
           proof - 
             have "KVSGSNonEmp gs'" using cmt I
               by (simp add: cl_commit_def KVSGSNonEmp_def KVSNonEmp_def invariant_list_def 
@@ -88,29 +62,37 @@ next
               by (auto simp add: full_view_wellformed)
           qed*) sorry
         next 
-          show \<open>view_wellformed (kvs_of_gs gs) (views_of_gs gs cl)\<close> (*using I
+          show \<open>view_wellformed (kvs_of_s gs) (views_of_s gs cl)\<close> (*using I
             by (auto 4 3 simp add: views_of_gs_def)*) sorry
         next 
-          show \<open>Tn_cl sn cl \<in> next_txids (kvs_of_gs gs) cl\<close> using cmt (*I
+          show \<open>Tn_cl sn cl \<in> next_txids (kvs_of_s gs) cl\<close> using cmt (*I
             by (auto simp add: cl_commit_def t_is_fresh)*) sorry
         next 
-          show \<open>fp_property F (kvs_of_gs gs) u''\<close> using cmt
-            apply (auto simp add: cl_commit_def fp_property_def view_snapshot_def)
+          show \<open>fp_property F (kvs_of_s gs) u''\<close>
+          proof -
+            have a: "\<And>k v. F k R = Some v \<Longrightarrow>
+              \<exists>t. svr_state (svrs gs k) (get_wtxn gs cl) = occ_s (Some (v, t)) (F k W)"
+              using cmt
+              apply (auto simp add: cl_commit_def)
+              by (smt UnI1 UnI2 eq_fst_iff map_option_eq_Some option.distinct(1))
+            show ?thesis using cmt
+              apply (auto simp add: cl_commit_def fp_property_def view_snapshot_def)
+              subgoal for k v
+                using a[of k v] apply auto sorry.
               (* Invariant: there is no timestamp inversion *)
-            subgoal for k a b
               (*apply (cases "svr_state (svrs gs k) (get_txn cl gs) = no_lock")
               subgoal by (auto simp add: NoLockFpInv_def invariant_list_def)
               subgoal by (smt (verit) RLockFpContentInv_def WLockFpContentInv_def
                                       empty_iff insertCI insertE invariant_listE o_apply 
                                       option.distinct(1) option.inject svr_vl_kvs_eq_lv) 
-              done*) sorry
-            sorry
+              done*)
+          qed
         next 
-          show \<open>kvs_of_gs gs' = update_kv (Tn_cl sn cl) F u'' (kvs_of_gs gs)\<close> using cmt (*I
+          show \<open>kvs_of_s gs' = update_kv (Tn_cl sn cl) F u'' (kvs_of_s gs)\<close> using cmt (*I
             by (auto 4 3 simp add: cl_commit_def kvs_of_gs_def update_kv_def 
                                    kvs_of_gs_cl_commit svr_cl_cl'_unchanged_def)*) sorry
         next 
-          show \<open>views_of_gs gs' = (views_of_gs gs)(cl := full_view o (updated_kvs gs cl ts))\<close> using cmt (*I
+          show \<open>views_of_s gs' = (views_of_s gs)(cl := full_view o (kvs_of_s gs'))\<close> using cmt (*I
             apply (auto simp add: cl_commit_def views_of_gs_def)
             apply (rule ext)
             by (auto simp add: cl_unchanged_defs intro: updated_is_kvs_of_gs')*) sorry
@@ -120,37 +102,52 @@ next
         by (simp only: ET_SER.trans_ET_ES_eq tapir_trans s_trans.simps sim_def med.simps)
     qed
   next
-    case (Cl_Prep x1 x2)
-    then show ?case apply (auto simp add: sim_defs tapir_trans_defs)
-      apply (rule ext)                
-      apply (auto simp add: update_kv_all_defs eligible_reads_def)
-      by (smt (verit) Collect_cong state_cl.distinct(4) version.cases version.update_convs(3))+
+    case (Cl_Prep x1 x2 x3 x4)
+    then show ?case
+      apply (auto simp add: sim_def tapir_trans_defs)
+      by (rule ext, auto simp add: sim_defs split: svr_state.split)+
+  next
+    case (Cl_Read_Resp x1 x2 x3 x4)
+    then show ?case
+      apply (auto simp add: sim_def tapir_trans_defs)
+      by (rule ext, auto simp add: sim_defs split: svr_state.split)+
   next
     case (Cl_Abort x)
-    then show ?case apply (auto simp add: sim_defs tapir_trans_defs)
-      apply (rule ext)                
-      apply (auto simp add: update_kv_all_defs eligible_reads_def)
-      by (smt (verit) Collect_cong state_cl.distinct(7) version.cases version.update_convs(3))+
+    then show ?case
+      apply (auto simp add: sim_def tapir_trans_defs)
+      by (rule ext, auto simp add: sim_defs split: svr_state.split)+
   next
-    case (Cl_ReadyA x)
-    then show ?case apply (auto simp add: sim_defs tapir_trans_defs)
-      apply (rule ext)                
-      apply (auto simp add: update_kv_all_defs eligible_reads_def)
-      by (smt (verit) Collect_cong state_cl.distinct(11) version.cases version.update_convs(3))+
+    case (Cl_ReadyC x1 x2)
+    then show ?case
+      apply (auto simp add: sim_defs tapir_trans_defs)
+      apply (rule ext, auto simp add: sim_defs split: svr_state.split) sorry
   next
-    case (TryPrep x1 x2 x3)
+    case (Cl_ReadyA x1 x2)
+    then show ?case
+      apply (auto simp add: sim_def tapir_trans_defs)
+      by (rule ext, auto simp add: sim_defs split: svr_state.split)+
+  next
+    case (Prep x1 x2 x3 x4)
+    then show ?case
+      apply (auto simp add: sim_defs tapir_trans_defs)
+      subgoal apply (elim ext_map_neqE, auto)
+        (*apply (auto simp add: sim_defs split: svr_state.split_asm option.split_asm)
+        apply (smt (verit) fun_upd_other fun_upd_same svr_conf.select_convs(1) svr_conf.surjective
+            svr_conf.update_convs(1) svr_state.distinct(13) svr_state.distinct(3))
+        apply (smt (verit) fun_upd_other fun_upd_same svr_conf.select_convs(1) svr_conf.surjective
+            svr_conf.update_convs(1) svr_state.distinct(17) svr_state.distinct(7))*) sorry
+      sorry
+  next
+    case (OCCCheck x1 x2 x3 x4 x5 x6)
     then show ?case sorry
   next
-    case (OCCCheck x1 x2 x3)
+    case (CommitR x1 x2 x3 x4)
     then show ?case sorry
   next
-    case (Commit x1 x2)
+    case (CommitW x1 x2 x3 x4)
     then show ?case sorry
   next
     case (Abort x1 x2)
-    then show ?case sorry
-  next
-    case (Cl_ReadyC x)
     then show ?case sorry
   qed simp                            
 qed
